---
title: Abstract Algebra by Pinter, Chapter 19
author: Amir Taaki
header-includes: |
    - \usepackage{mathrsfs}
    - \usepackage{mathtools}
    - \usepackage{extpfeil}
    - \DeclareMathOperator\ker{ker}
    - \DeclareMathOperator\ord{ord}
    - \DeclareMathOperator\gcd{gcd}
    - \DeclareMathOperator\lcm{lcm}
    - \DeclareMathOperator\mod{mod}
abstract: Chapter 19 on Quotient Rings
---

# A. Examples of Quotient Rings

## Q1

$$A = \mathbb{Z}_{10}, J = \{ 0, 5 \}$$

\begin{align*}
J = J + 0 &= \{ 0, 5 \} \\
J + 1 &= \{ 1, 6 \} \\
J + 2 &= \{ 2, 7 \} \\
J + 3 &= \{ 3, 8 \} \\
J + 4 &= \{ 4, 9 \}
\end{align*}

\begin{tabular}{c | c c c c c c c c c}
    $+$ & J   & J + 1 & J + 2 & J + 3 & J + 4 \\
    \cline{1-6}
J     &   J   & J + 1 & J + 2 & J + 3 & J + 4 \\
J + 1 & J + 1 & J + 2 & J + 3 & J + 4 & J     \\
J + 2 & J + 2 & J + 3 & J + 4 & J     & J + 1 \\
J + 3 & J + 3 & J + 4 & J     & J + 1 & J + 2 \\
J + 4 & J + 4 & J     & J + 1 & J + 2 & J + 3 \\
\end{tabular}

\begin{tabular}{c | c c c c c c c c c}
$\cdot$ & J   & J + 1 & J + 2 & J + 3 & J + 4 \\
    \cline{1-6}
J     &   J   & J     & J     & J     & J     \\
J + 1 & J     & J + 1 & J + 2 & J + 3 & J + 4 \\
J + 2 & J     & J + 2 & J + 4 & J + 1 & J + 3 \\
J + 3 & J     & J + 3 & J + 1 & J + 4 & J + 2 \\
J + 4 & J     & J + 4 & J + 3 & J + 2 & J + 1 \\
\end{tabular}

## Q2

$$A = P_3, J = \{ \varnothing, \{a\}\}$$

\begin{align*}
J = J + 0 &= \{ \varnothing, \{a \}\} \\
J + \{ b \} &= \{ \{b\}, \{a, b \}\} \\
J + \{ c \} &= \{ \{c\}, \{a, c \}\} \\
J + \{ b, c \} &= \{ \{b, c\}, \{a, b, c \}\} \\
\end{align*}

\begin{tabular}{c | c c c c c c c c c}
    $+$ &       J         & J + \{b\}   & J + \{c\}   & J + \{b,c\} \\
    \cline{1-5}    
J           &   J         & J + \{b\}   & J + \{c\}   & J + \{b,c\} \\
J + \{b\}   & J + \{b\}   & J           & J + \{b,c\} & J + \{c\}   \\
J + \{c\}   & J + \{c\}   & J + \{b,c\} & J           & J + \{b\}   \\
J + \{b,c\} & J + \{b,c\} & J + \{c\}   & J + \{b\}   & J           \\
\end{tabular}

\begin{tabular}{c | c c c c c c c c c}
$\cdot$ &       J         & J + \{b\}   & J + \{c\}   & J + \{b,c\} \\
    \cline{1-5}    
J           & J           & J           & J           & J           \\
J + \{b\}   & J           & J + \{b\}   & J           & J + \{b\}   \\
J + \{c\}   & J           & J           & J + \{c\}   & J + \{c\}   \\
J + \{b,c\} & J           & J + \{b\}   & J + \{c\}   & J + \{b,c\} \\
\end{tabular}

## Q3

$$A = \mathbb{Z}_2 \times \mathbb{Z}_6, J = \{(0, 0), (0, 2), (0, 4)\}$$

\begin{align*}
J &= \{(0, 0), (0, 2), (0, 4)\} \\
J + (0, 1) &= \{(0, 1), (0, 3), (0, 5)\} \\
J + (1, 0) &= \{(1, 0), (1, 2), (1, 4)\} \\
J + (1, 1) &= \{(1, 1), (1, 3), (1, 5)\} \\
\end{align*}

\begin{tabular}{c | c c c c c c c c c}
    $+$ &       J         & J + (0,1)   & J + (1,0)   & J + (1,1)   \\
    \cline{1-5}    
J           &   J         & J + (0,1)   & J + (1,0)   & J + (1,1)   \\
J + (0,1)   & J + (0,1)   & J           & J + (1,1)   & J + (1,0)   \\
J + (1,0)   & J + (1,0)   & J + (1,1)   & J           & J + (0,1)   \\
J + (1,1)   & J + (1,1)   & J + (1,0)   & J + (0,1)   & J           \\
\end{tabular}

\begin{tabular}{c | c c c c c c c c c}
$\cdot$ &       J         & J + (0,1)   & J + (1,0)   & J + (1,1)   \\
    \cline{1-5}    
J           &   J         & J           & J           & J           \\
J + (0,1)   & J           & J + (0,1)   & J           & J + (0,1)   \\
J + (1,0)   & J           & J           & J + (1,0)   & J + (1,0)   \\
J + (1,1)   & J           & J + (0,1)   & J + (1,0)   & J + (1,1)   \\
\end{tabular}

# B. Examples of the Use of the FHT

## Q1

$$f(x) = x \mod 5$$
$$\ker f = \{ 0, 5, 10, 15 \} = \langle 5 \rangle$$
$$\mathbb{Z}_5 \cong \mathbb{Z}_{20} / \langle 5 \rangle$$

\begin{align*}
J = J + 0 &= \{ 0, 5, 10, 15 \} \\
J + 1 &= \{ 1, 6, 11, 16 \} \\
J + 2 &= \{ 2, 7, 12, 17 \} \\
J + 3 &= \{ 3, 8, 13, 18 \} \\
J + 4 &= \{ 4, 9, 14, 19 \}
\end{align*}

\begin{tabular}{c | c c c c c c c c c}
    $+$ & J   & J + 1 & J + 2 & J + 3 & J + 4 \\
    \cline{1-6}
J     &   J   & J + 1 & J + 2 & J + 3 & J + 4 \\
J + 1 & J + 1 & J + 2 & J + 3 & J + 4 & J     \\
J + 2 & J + 2 & J + 3 & J + 4 & J     & J + 1 \\
J + 3 & J + 3 & J + 4 & J     & J + 1 & J + 2 \\
J + 4 & J + 4 & J     & J + 1 & J + 2 & J + 3 \\
\end{tabular}

\begin{tabular}{c | c c c c c c c c c}
$\cdot$ & J   & J + 1 & J + 2 & J + 3 & J + 4 \\
    \cline{1-6}
J     &   J   & J     & J     & J     & J     \\
J + 1 & J     & J + 1 & J + 2 & J + 3 & J + 4 \\
J + 2 & J     & J + 2 & J + 4 & J + 1 & J + 3 \\
J + 3 & J     & J + 3 & J + 1 & J + 4 & J + 2 \\
J + 4 & J     & J + 4 & J + 3 & J + 2 & J + 1 \\
\end{tabular}

Tables are exact same for mod 5.

## Q2

$$f(x) = x \mod 3$$
$$\ker f = \{ 0, 3 \} = \langle 3 \rangle$$
$$\mathbb{Z}_3 \cong \mathbb{Z}_6 / \langle 3 \rangle$$

\begin{align*}
J = J + 0 &= \{ 0, 3 \} \\
J + 1 &= \{ 1, 4 \} \\
J + 2 &= \{ 2, 5 \} \\
\end{align*}

\begin{tabular}{c | c c c c c c c c c}
    $+$ & J   & J + 1 & J + 2 \\
    \cline{1-4}
J     &   J   & J + 1 & J + 2 \\
J + 1 & J + 1 & J + 2 & J  \\
J + 2 & J + 2 & J     & J + 1 \\
\end{tabular}

\begin{tabular}{c | c c c c c c c c c}
$\cdot$ & J   & J + 1 & J + 2 \\
    \cline{1-4}
J     &   J   & J     & J     \\
J + 1 & J     & J + 1 & J + 2 \\
J + 2 & J     & J + 2 & J + 1 \\
\end{tabular}

Tables are exact same for mod 3.

## Q3

$$P_2 = \{ \varnothing, \{a\}, \{b\}, \{a, b\}\}$$
$$P_3 = \{ \varnothing, \{a\}, \{b\}, \{c\}, \{a,b\}, \{a,c\}, \{b,c\}, \{a,b,c\} \}$$
\begin{align*}
K = K + \varnothing &= \{ \varnothing, \{ c \} \} \\
K + \{ a \} &= \{ \{ a \}, \{ a, c \} \} \\
K + \{ b \} &= \{ \{ b \}, \{ b, c \} \} \\
K + \{ a, b \} &= \{ \{ a, b \}, \{ a, b, c \} \} \\
\end{align*}
$$f(X) = X \cap \{ a, b \}$$
$$f : P_3 \rightarrow P_2$$
$$P_2 \cong P_3 / \langle \{ \varnothing, \{ c \} \} \rangle$$

\begin{tabular}{c | c c c c c c c c c}
    $+$     & K           & K + \{a\}   & K + \{b\}   & K + \{a,b\} \\
    \cline{1-5}
K           &   K         & K + \{a\}   & K + \{b\}   & K + \{a,b\} \\
K + \{a\}   & K + \{a\}   & K           & K + \{a,b\} & K + \{b\}   \\
K + \{b\}   & K + \{b\}   & K + \{a,b\} & K           & K + \{a\}   \\
K + \{a,b\} & K + \{a,b\} & K + \{b\}   & K + \{a\}   & K           \\
\end{tabular}

\begin{tabular}{c | c c c c c c c c c}
$\cdot$     & K           & K + \{a\}   & K + \{b\}   & K + \{a,b\} \\
    \cline{1-5}
K           & K           & K           & K           & K           \\
K + \{a\}   & K           & K + \{a\}   & K           & K + \{a\}   \\
K + \{b\}   & K           & K           & K + \{b\}   & K + \{b\}   \\
K + \{a,b\} & K           & K + \{a\}   & K + \{b\}   & K + \{a,b\} \\
\end{tabular}

## Q4

$$f: \mathbb{Z}_2 \times \mathbb{Z}_2 \rightarrow \mathbb{Z}_2$$
$$f((x, y)) = x$$
$$K = \{ (0,0), (0, 1) \}$$
$$K + (1, 0) = \{ (1,0), (1,1) \}$$

\begin{tabular}{c | c c c c c c c c c}
    $+$     & K           & K + (1,0) \\
    \cline{1-3}                
K           &   K         & K + (1,0) \\
K + (1,0)   & K + (1,0)   & K         \\
\end{tabular}

\begin{tabular}{c | c c c c c c c c c}
$\cdot$     & K           & K + (1,0) \\
    \cline{1-3}                
K           &   K         & K         \\
K + (1,0)   & K           & K + (1,0) \\
\end{tabular}

# C. Quotient Rings and Homomorphic Images in $\mathcal{F}(\mathbb{R})$

## Q1

$$\phi : \mathcal{F}(\mathbb{R}) \rightarrow \mathbb{R} \times \mathbb{R}$$
$$\phi(f) = (f(0), f(1))$$

1. $\phi(f + g) = ((f + g)(0), (f + g)(1)) = (f(0), f(1)) + (g(0), g(1)) = \phi(f) + \phi(g)$
2. $\phi(f \cdot g) = ((f \cdot g)(0), (f \cdot g)(1)) = (f(0), f(1))(g(0), g(1)) = \phi(f)\phi(g)$

Let $f(x) = (a - b)x + b$, then $f \in \mathcal{F}(\mathbb{R})$, $f(0) = b$ and $f(1) = a$. Thus functions of this form can represent any value in $\mathbb{R} \times \mathbb{R}$ and so the homomorphism $\phi$ is *onto* $\mathbb{R} \times \mathbb{R}$.

$$K = \{ f \in \mathcal{F}(\mathbb{R}) : f(0) = 0 \text{ and } f(1) = 0 \}$$

## Q2

$$J = \{ f \in \mathcal{F}(\mathbb{R}) : f(0) = 0 \text{ and } f(1) = 0 \}$$

Thus $J$ is the kernel of the homomorphism $\phi$. The kernel is also an ideal of $\mathcal{F}(\mathbb{R})$, so
$$\mathcal{F}(\mathbb{R}) / J \cong \mathbb{R} \times \mathbb{R}$$

## Q3

$$\phi: \mathcal{F}(\mathbb{R}) \rightarrow \mathcal{F}(\mathbb{Q}, \mathbb{R})$$
$$\phi(f) = f_{\mathbb{Q}} = \text{ the restriction of } f \text{ to } \mathbb{Q}$$

$\phi$ is onto because $\forall g \in \mathcal{F}(\mathbb{Q}, \mathbb{R}), \exists f \in \mathcal{F}(\mathbb{R}) : g = f_{\mathbb{Q}}$. $\phi$ is a homomorphism since $\phi(f \cdot g) = \phi(f) \cdot \phi(g)$ and $\phi(f + g) = \phi(f) + \phi(g)$.

$$K = \{ f \in \mathcal{F}(\mathbb{R}) : f(x) = 0 \}$$

## Q4

$J$ is also the kernel of $\mathcal{F}(\mathbb{R})$, which means it is also an ideal. Thus
$$\mathcal{F}(\mathbb{R}) / J \cong \mathcal{F}(\mathbb{Q})$$

# D. Elementary Applications of the Fundamental Homomorphism Theorem

## Q1

Note that ring is commutative then
$$(x + y)^2 = x(x + y) + y(x + y) = x^2 + xy + yx + y^2 = x^2 + 2xy + y^2 = x^2 + y^2$$

So $h(x) = x^2$ is a homomorphism since $h(x + y) = x^2 + y^2 = h(x) + h(y)$ and $h(xy) = x^2 y^2 = h(x) h(y)$

$$J = \{x \in A : x^2 = 0 \}$$
$$B = \{ x^2 : x \in A \}$$

$h$ is a homomorphism from $A$ to $B$ and the kernel is $J$
$$A/J \cong B$$

## Q2

$h(x) = 3x$ is a homomorphism because $h(x + y) = 3x + 3y = h(x) + h(y)$ and $h(xy) = h(x) h(y)$ because
$$h(xy) = 3xy = 6xy + 3xy = (3x)(3y) = h(x)h(y)$$

$J = \{ x : 3x = 0 \}$ is the kernel and thus ideal of $h$. $B = \{ 3x : x \in A \}$ is a subring of $A$ by the homomorphism shown above
$$A/J \cong B$$

## Q3

$$\pi_a(xy) = axy = a^2 xy = (ax)(ay) = \pi_a(x)\pi_a(y)$$
$$\pi_a(x + y) = a(x + y) = ax + ay = \pi_a(x) + \pi_a(y)$$
$$I_a = \{ x \in A : ax = 0 \} = \ker \pi_a$$
$$\pi_a(1) = a$$
$$\pi_a(x) = \pi_a(x \cdot 1) = a + \cdots + a \in \langle a \rangle$$
$$\pi_a : A \rightarrow \langle a \rangle$$
$$A / I_a \cong \langle a \rangle$$

## Q4

$$\phi(ab) = \pi_{ab} = \pi_a \pi_b = \phi(a) \phi(b)$$
$$\phi(a + b) = \pi_{a + b} = \pi_a + \pi_b = \phi(a) + \phi(b)$$
$$I = \{ x \in A : ax = 0, \forall a \in A \}$$
$$\pi_a(x) = ax$$
$$\bar{A} = \{ \pi_a : a \in A \}$$
$$\phi(a) = \pi_a$$
$$\ker \phi = \{ x \in A : \phi(x) = \pi_0 \}$$
$$\forall a \in A \qquad \pi_0(a) = 0$$
$$\therefore \ker \phi = I$$
$$\phi : A \rightarrow \bar{A}$$
$$A/I \cong \bar{A}$$

