---
title: Abstract Algebra by Pinter, Chapter 31
author: Amir Taaki
header-includes: |
    - \usepackage{mathrsfs}
    - \usepackage{mathtools}
    - \usepackage{extpfeil}
    - \DeclareMathOperator\ker{ker}
    - \DeclareMathOperator\ord{ord}
    - \DeclareMathOperator\gcd{gcd}
    - \DeclareMathOperator\lcm{lcm}
    - \DeclareMathOperator\char{char}
    - \DeclareMathOperator\max{max}
    - \DeclareMathOperator\ran{ran}
    - \DeclareMathOperator\deg{deg}
    - \DeclareMathOperator\dim{dim}
    - \newcommand{\mod}[1]{\ (\mathrm{mod}\ #1)}
    - \newcommand{\repr}[1]{\overline{#1}}
    - \newcommand{\leg}[2]{\left(\frac{#1}{#2}\right)}
    - \let\vec\mathbf
abstract: Chapter 31 on Galois Theory Preamble
---

Note that root field is called splitting field in other texts.

# A. Examples of Root Fields over $\mathbb{Q}$

## Q1

```python
sage: solve(x^2 - 2*x - 2, x)
[x == -sqrt(3) + 1, x == sqrt(3) + 1]
sage: solve(x^2 + 1, x)
[x == -I, x == I]
```

## Q2

Possible roots for $x^2 - 3$ are $\pm 1, \pm 3$.

```python
sage: p = lambda x: x^2 - 3
sage: p(-1), p(1), p(-3), p(3)
(-2, -2, 6, 6)
```

So it is irreducible.

For $x^2 - 2x - 2$ we can use Eisenstein's irreducibility criteria.

```python
sage: solve(x^2 - 3, x)
[x == -sqrt(3), x == sqrt(3)]
sage: solve(x^2 - 2*x - 2, x)
[x == -sqrt(3) + 1, x == sqrt(3) + 1]
```

Root field is $\mathbb{Q}(\sqrt{3})$.

## Q3

```python
sage: solve(x^4 - 2, x)
[x == I*2^(1/4), x == -2^(1/4), x == -I*2^(1/4), x == 2^(1/4)]
```

Therefore the root field is $\mathbb{Q}(2^{\frac{1}{4}}, i)$

Since $\mathbb{Q}(2^{\frac{1}{4}}) \subseteq \mathbb{R}$, then the root field of $x^4 - 2$ over $\mathbb{R}$ is $\mathbb{R}(i)$.

## Q4

```python
sage: solve(x^4 - 2*x^2 + 9, x)
[x == -sqrt(2*I*sqrt(2) + 1), x == sqrt(2*I*sqrt(2) + 1), x == -sqrt(-2*I*sqrt(2) + 1), x == sqrt(-2*I*sqrt(2) + 1)]
```

Root field is $\mathbb{Q}(i, \sqrt{2})$.

```python
sage: solve(x^2 - 2*sqrt(2)*x + 3, x)
[x == sqrt(2) - I, x == sqrt(2) + I]
```

Root field is $\mathbb{Q}(i, \sqrt{2})$.

## Q5

```python
sage: c
sqrt(3) + I
sage: ((c^2 - 2)^2).expand()
-12
sage: ((x^2 - 2)^2
....: ).expand()
x^4 - 4*x^2 + 4
sage: x^4 - 4*x^2 + 4 + 12
x^4 - 4*x^2 + 16
sage: solve(x^4 - 4*x^2 + 4 + 12, x)
[x == -sqrt(2*I*sqrt(3) + 2), x == sqrt(2*I*sqrt(3) + 2), x == -sqrt(-2*I*sqrt(3) + 2), x == sqrt(-2*I*sqrt(3) + 2)]

```

So there are roots $-2\sqrt{3}i - 2$ and $2\sqrt{3}i - 2$.

And $x^2 - 3$ for $b(x)$.

```python
sage: c = sqrt(2) + sqrt(3)
sage: (c^2).expand()
2*sqrt(3)*sqrt(2) + 5
sage: (((c^2).expand() - 5)^2).expand()
24
sage: ((x^2 - 5)^2).expand()
x^4 - 10*x^2 + 25
sage: solve(x^4 - 10*x^2 + 1, x)
[x == -sqrt(2*sqrt(6) + 5), x == sqrt(2*sqrt(6) + 5), x == -sqrt(-2*sqrt(6) + 5), x == sqrt(-2*sqrt(6) + 5)]
```

Remembering that $\sqrt{6} = \sqrt{2} \sqrt{3}$.

## Q6

All of them are valid root fields except the cube root one.

# B. Examples of Root Fields over $\mathbb{Z}_p$

## Q1

```python
sage: R.<x> = IntegerModRing(3)[]
sage: f = x^3 + 2*x + 1
sage: S.<u> = R.extension(f)
sage: (x - u)*(x - (u + 1))*(x - (u + 2))
x^3 + 2*x + 1
```

List the elements:

```python
sage: S = R.quotient(x^3 + 2*x + 1, 'u')
sage: len(S)
27
sage: list(S)
[0,
 1,
 2,
 u,
 u + 1,
 u + 2,
 2*u,
 2*u + 1,
 2*u + 2,
 u^2,
 u^2 + 1,
 u^2 + 2,
 u^2 + u,
 u^2 + u + 1,
 u^2 + u + 2,
 u^2 + 2*u,
 u^2 + 2*u + 1,
 u^2 + 2*u + 2,
 2*u^2,
 2*u^2 + 1,
 2*u^2 + 2,
 2*u^2 + u,
 2*u^2 + u + 1,
 2*u^2 + u + 2,
 2*u^2 + 2*u,
 2*u^2 + 2*u + 1,
 2*u^2 + 2*u + 2]
```

Roots of $a(x)$ are $u, u + 1, u + 2$.

Root field is therefore $\mathbb{Z}_3(u)$.

## Q2

```python
sage: S = R.quotient(x^2 + x + 2, 'u')
sage: list(S)
[0, 1, 2, u, u + 1, u + 2, 2*u, 2*u + 1, 2*u + 2]
```

Utilize the fact that $u^2 = - u - 2 = 2u + 1$, we can make the addition and multiplication tables.

```python
sage: from sage.matrix.operation_table import OperationTable
sage: OperationTable(S, operation=operator.add)
+  a b c d e f g h i
 +------------------
a| a b c d e f g h i
b| b c a e f d h i g
c| c a b f d e i g h
d| d e f g h i a b c
e| e f d h i g b c a
f| f d e i g h c a b
g| g h i a b c d e f
h| h i g b c a e f d
i| i g h c a b f d e

sage: OperationTable(S, operation=operator.mul)
*  a b c d e f g h i
 +------------------
a| a a a a a a a a a
b| a b c d e f g h i
c| a c b g i h d f e
d| a d g h b e f i c
e| a e i b f g c d h
f| a f h e g c i b d
g| a g d f c i h e b
h| a h f i d b e c g
i| a i e c h d b g f
```

Roots are: $u, 2u + 2$ (figured by substitution)

Root field: $\mathbb{Z}_3(u)$

## Q3

Root field will be all combos of polynomials over $\mathbb{Z}_2$ of degree 2 polynomials.

```python
sage: R.<x> = IntegerModRing(2)[]
sage: S = R.quotient(x^3 + x^2 + 1, 'u')
sage: list(S)
[0, 1, u, u + 1, u^2, u^2 + 1, u^2 + u, u^2 + u + 1]
```

In $\mathbb{Z}_2$, $-1 = 1$ so $u^3 = u^2 + 1$.

```python
sage: OperationTable(S, operation=operator.add)
+  a b c d e f g h
 +----------------
a| a b c d e f g h
b| b a d c f e h g
c| c d a b g h e f
d| d c b a h g f e
e| e f g h a b c d
f| f e h g b a d c
g| g h e f c d a b
h| h g f e d c b a

sage: OperationTable(S, operation=operator.mul)
*  a b c d e f g h
 +----------------
a| a a a a a a a a
b| a b c d e f g h
c| a c e g f h b d
d| a d g f b c h e
e| a e f b h d c g
f| a f h c d g e b
g| a g b h c e d f
h| a h d e g b f c
```

```python
sage: R.<x> = IntegerModRing(2)[]
sage: f = x^3 + x^2 + 1
sage: S.<u> = R.extension(f)
...
sage: f(u)
0
sage: f(u^2)
0
sage: f(u^2 + u + 1)
0
sage: (x - u)*(x - u^2)*(x - (u^2 + u + 1))
x^3 + x^2 + 1
```

Root field: $\mathbb{Z}_3(u)$

## Q4

```python
sage: f = x^3 + x + 1
sage: S.<u> = R.extension(f)
sage: f(u)
0
sage: f(u + 1)
u^2 + u
sage: f(u^2)
0
sage: f(u^2 + 1)
u
sage: f(u^2 + u)
0
sage: f(u^2 + u + 1)
u^2
```

Roots are $u, u^2, u^2 + u$.

## Q5

```python
sage: R.<x> = IntegerModRing(3)[]
sage: f = x^3 + x^2 + x + 2
sage: S.<u> = R.extension(f)
sage: f(u)
0
sage: f(u + 1)
2*u
sage: f(u + 2)
u + 2
sage: f(u^2)
u^2
sage: f(u^2 + 1)
0
sage: f(u^2 + 2)
2*u^2 + 2
sage: f(u^2 + u)
2*u^2 + u
sage: f(u^2 + u + 1)
u^2
sage: f(u^2 + 2*u)
2*u^2 + 2*u
sage: f(u^2 + 2*u + 1)
u^2
sage: f(u^2 + u + 2)
2*u + 2
sage: f(u^2 + 2*u + 2)
u + 2
sage: f(2*u)
2*u^2 + 1
sage: f(2*u + 1)
2*u^2 + u + 1
sage: f(2*u + 2)
2*u^2 + 2*u
sage: f(2*u^2)
2*u^2 + u + 2
sage: f(2*u^2 + 1)
u + 2
sage: f(2*u^2 + 2)
u^2 + u + 1
sage: f(2*u^2 + u)
u^2 + 1
sage: f(2*u^2 + 2*u)
2*u^2 + 2*u
sage: f(2*u^2 + u + 1)
2*u^2 + 2*u + 1
sage: f(2*u^2 + u + 2)
u
sage: f(2*u^2 + 2*u + 1)
0
```

I think the answer in the book is wrong since

```python
sage: R.<x> = IntegerModRing(3)[]
sage: f = x^3 + x^2 + x + 2
sage: S.<u> = R.extension(f)
sage: u^3 + u^2 + u + 2
0
sage: f(u^2 + 1)
0
sage: f(2*u^2 + 2*u + 1)
0
sage: (x - u)*(x - (u^2 + 1))*(x - (2*u^2 + 2*u + 1))
x^3 + x^2 + x + 2
```

We can even substitute these roots into $q(x)$ which is claimed to be irreducible

```python
sage: a = lambda x: (x^2 + (u + 1)*x + (u^2 + u + 1))
sage: a(u^2 + 1)
0
sage: a(2*u^2 + 2*u + 1)
0
```

Roots are: $u, u^2 + 1, 2u^2 + 2u + 1$.

Basis is $\{ u^2, u, 1 \}$.

# C. Short Questions Relating to Root Field

## Q1

The basis for a degree 2 extension $\mathbb{F}(c)$ is $\{c, 1\}$ with $c^2 \in \mathbb{F}$. This includes $-c$ and so $\mathbb{F}(c)$ is the root field for $(x + c)(x - c) = x^2 - c^2$.

The question I assume is asking to prove every degree 2 field extension is [normal](https://en.wikipedia.org/wiki/Normal_extension). So since $c \in F(c)$, then we can divide the polynomial by $(x - c)$, leaving a degree 1 polynomial $(x - \alpha) \in F(c)[x]$ or that $\alpha \in F(c)$.

## Q2

$a(x)$ as a polynomial of degree $n$ over a finite field will have $n$ distinct roots. All roots $c_1, \dots, c_n \in K$ and form a root field over $F$. Assume some roots are in $I$, then the roots of $a(x)$ are still the same, and so $K$ forms a root field over $I$ as well.

## Q3

Any polynomial can be factored into a linear combination of complex roots. This means $\mathbb{C}$ is the root field of every polynomial. Since polynomials can also have root fields contained in $\mathbb{R}$, and $\mathbb{R} \subset \mathbb{C}$, this means the root field is either $\mathbb{R}$ or $\mathbb{C}$ of every polynomial.

## Q4

This question is impossible. See the answer [here](https://math.stackexchange.com/questions/850518/splitting-field-of-cubic-polynomial-over-the-rationals).

## Q5

As per the back of the book, we just need to show that $F(d_1, d_2) = F(c)$ and that it's the splitting field.

\begin{align*}
d_1^2 &= \frac{a^2}{4} - b \\
d_2^2 &= \frac{a}{2} + d_1 \\
      &= \frac{a}{2} + \sqrt{\frac{a^2}{4} - b}
\end{align*}

Roots of $p(x)$ are $\pm \sqrt{\frac{a}{2} \pm d_1}$. We know that $\frac{a}{2} \pm d_1 \in F(d_1)$.

$[F(d_1): F] = 2$. Every extension of degree 2 is a root field from 31C1 above.

## Q6

$$\sigma_c(a(x)) = a(c)$$
$$\ker \sigma_c = \{ a(x): a(c) = 0 \}$$
Every ideal of a field [is principal](https://sharmaeklavya2.github.io/theoremdep/nodes/polynomials/every-ideal-is-principal.html), so $J = \langle p(x) \rangle$.
For some $a(x) \in J$, $a(x)$ is a multiple of $p(x)$.
$$\sigma_c : F[x] \rightarrow F$$
so $F(c)$ contains $p(x)$ since the ideal $J$ contains all polynomials with $c$ as their root, and all polys are a multiple of $p(x)$.

## Q7

From the previous argument $p(x)$ is the lowest degree polynomial in $J$ and hence irreducible.
Otherwise $p(c) = f(c)g(c) = 0 \implies f(c) = 0 \textrm{ or } g(c) = 0$
which would be a contradiction since it implies there would be a lower degree polynomial in $J$.
Every root field is a simple extension $F(c)$, we can convert a polynomial with roots $a, b$ to one with $c$ from theorem 2 in this chapter.

## Q8

Give an isomorphism $h(x)$ which fixes F, and a polynomial
$$a(x) = a_0 + a_1 x + \cdots + a_n x^n$$
We can see that where $c$ is an algebraic root in $K$, then
\begin{align*}
a(h(c)) &= a_0 + a_1 h(c) + \cdots + a_n h(c^n) \\
&= h(a(c)) = h(0) = 0
\end{align*}
So also $h(c)$ is a root of $a(x)$ and the isomorphism simply permutes roots since it sends unique elements of $K$ to $K'$.
We also observe that the mapping is one to one, fixing $F$, permuting roots, and that $h: K \rightarrow K$.
$$h(\{c_1, \dots, c_n\}) = \{ c_1, \dots, c_n \}$$

Since the polynomial $a(x)$ is irreducible over $F$, and $K$ being a finite extension can be reduced to a simple extension $F(c) = K$, where $c$ is a root of $a(x)$, which means that
$$F(c) \cong F / \langle a(x) \rangle$$
which forms a vector space of $\deg a(x) = n \implies [K:F] = n$.

Given another polynomial $b(x)$ where $b(c) = 0 : c \in K \implies b(h(c)) = 0 \implies$ K is the splitting field for $b(x)$.
This means $b(x)$ is split completely by $K$ into linear factors.

Note, this means every polynomial of degree $n$ which has a root in $K$ makes $K$ its splitting field. The converse does not hold. An irreducible polynomial of degree $n$ does not necessarily have a splitting field of degree $n$. See [this answer](https://math.stackexchange.com/questions/1199018/show-for-an-irreducible-polynomial-fx-in-fx-of-degree-n-n-divides).

## Q9

First we prove this for an irreducible polynomial $p(x)$ with $n = \deg p(x)$ roots of the form $c_1, \dots, c_n$. Inductively adjoining $c_1$ to $F$ forms a field $F(c_1)$ such that $[F(c_1):F] = n$ with a basis $\{ 1, c_1, \dots, c_1^{n - 1} \}$. Dividing $p(x)$ by $(x - c_1)$ leaves a polynomial $q(x)$ with degree $n - 1$ and adjoining the second root to $F(c_1)$ forms a field extension with degree $[F(c_1, c_2):F(c_1)] = n - 1$. Proceeding in this way, we obtain a maximum order of $n!$.

The polynomial $a(x)$ is reducible to $n$ irreducible factors $a(x) = p_1(x) p_2(x) \cdots p_n(x)$ where $\deg p_i(x) = k_i$. Each of these fields forms a simple extension $F(c_1, \cdots, c_n)$, where $[F(c_1, \cdots, c_n):F] = [F(c_1, \cdots, c_n):F(c_1, \cdots, c_{n - 1})]\cdots[F(c_1):F] = k_n \cdot k_{n - 1} \cdots k_1$.

Since $\deg a(x) = N$ and $k_1 + \cdots k_n$, so $[K:F] \mid k_1! \cdots k_n!$.

From the binomial formula, given $n = k + l$, then there's an integer $z$ such that
$$z = \frac{n!}{k!l!} \implies n! = z k! l!$$                                   
So therefore given $n = k_1 + \cdots + k_n$, we can see that $x \mid k_1! \cdots k_n! \implies x \mid n!$

# D. Reducing Iterated Extensions to Simple Extensions

## Q1

### a

$$\mathbb{Q}(\sqrt{2}, i\sqrt{3}) = \mathbb{Q}(\sqrt{2} + i\sqrt{3})$$
$$c = \sqrt{2} + i\sqrt{3}$$
$$[\mathbb{Q}(c):\mathbb{Q}] = 4$$
$$\implies \sqrt{2} = a_0 + a_1 c + a_2 c^2 + a_3 c^3$$
$$c^2 = 2i \sqrt{6} - 1 \implies i\sqrt{6} \in \mathbb{Q}(c)$$
$$c^3 = 4i\sqrt{3} - \sqrt{2} - 6\sqrt{2} - i\sqrt{3} = 3i\sqrt{3} - 7\sqrt{2}$$
$$c^3 + 7c = 10i\sqrt{3} \implies i\sqrt{3} \in \mathbb{Q}(c)$$
Same can be shown for $\sqrt{2}$.

### b

$$(\sqrt[6]{2})^3 = \sqrt{2}, (\sqrt[6]{2})^2 = \sqrt[3]{2}$$
$$\implies \mathbb{Q}(\sqrt{2}, \sqrt[3]{2}) = \mathbb{Q}(\sqrt[6]{2})$$

## Q2

The roots of $x^2 - 2x - 1$ by completing the square are $\pm \sqrt{2} + 1$.

For a cubic with real coefficients in a field, it either has all real roots or 2 complex roots. By differentiating and sketching the curve where it's increasing or decreasing, we see that this cubic has two complex roots.

According to the **Complex Conjugate Theorem**, if $x = a + ib$ is a solution to a polynomial with real coefficients, then so is $x = a - ib$.

Thus we conclude that $\mathbb{Q}(a, b) = \mathbb{Q}(a + b)$ where $a$ is a complex root of $x^3 - x - 1$.

## Q3

These factors are all linearly independent so $c = \sqrt{2} + \sqrt{3} + \sqrt{-5}$.

## Q4

From C6, because $\sqrt{2}$ and $\sqrt{3}$ are independent, the basis is $\{ 1, \sqrt{2}, \sqrt{3}, \sqrt{6} \}$ and so the minimum polynomial has degree 4.

```python
sage: # We let x = sqrt(2) + sqrt(3), so now we square it on both sides
sage: (sqrt(2) + sqrt(3))^2
(sqrt(3) + sqrt(2))^2
sage: ((sqrt(2) + sqrt(3))^2).expand()
2*sqrt(3)*sqrt(2) + 5
sage: # so now (x^2 - 5) = 2*sqrt(3)*sqrt(2)
sage: # lets square again both sides
sage: (2*sqrt(3)*sqrt(2))**2
24
sage: ((x^2 - 5)^2).expand()
x^4 - 10*x^2 + 25
sage: ((x^2 - 5)^2).expand() - 24
x^4 - 10*x^2 + 1
```

## Q5

The minimum polynomial will now have degree 8.

```python
sage: x - sqrt(2) == sqrt(3) + I*sqrt(5)
x - sqrt(2) == I*sqrt(5) + sqrt(3)
sage: (x - sqrt(2) == sqrt(3) + I*sqrt(5))^2
(x - sqrt(2))^2 == (I*sqrt(5) + sqrt(3))^2
sage: ((x - sqrt(2) == sqrt(3) + I*sqrt(5))^2).expand()
x^2 - 2*sqrt(2)*x + 2 == 2*I*sqrt(5)*sqrt(3) - 2
sage: ((x - sqrt(2) == sqrt(3) + I*sqrt(5))^2).expand() + 2*sqrt(2)*x
x^2 + 2 == 2*sqrt(2)*x + 2*I*sqrt(5)*sqrt(3) - 2
sage: p = ((x - sqrt(2) == sqrt(3) + I*sqrt(5))^2).expand() + 2*sqrt(2)*x
sage: p
x^2 + 2 == 2*sqrt(2)*x + 2*I*sqrt(5)*sqrt(3) - 2
sage: p += 2
sage: p
x^2 + 4 == 2*sqrt(2)*x + 2*I*sqrt(5)*sqrt(3)
sage: (p^2).expand()
x^4 + 8*x^2 + 16 == 8*I*sqrt(5)*sqrt(3)*sqrt(2)*x + 8*x^2 - 60
sage: (p^2).expand() + 60 - 8*x^2
x^4 + 76 == 8*I*sqrt(5)*sqrt(3)*sqrt(2)*x
sage: p = (p^2).expand() + 60 - 8*x^2
sage: (p^2).expand()
x^8 + 152*x^4 + 5776 == -1920*x^2
sage: (p^2).expand() + 1920*x^2
x^8 + 152*x^4 + 1920*x^2 + 5776 == 0
sage: p = x^8 + 152*x^4 + 1920*x^2 + 5776
sage: p(x = sqrt(2) + sqrt(3) + I*sqrt(5)).expand()
0
```

# E. Roots of Unity and Radical Extensions

## Q1

The roots of $x^n - 1$ are $1, \omega, \dots, \omega^{n - 1}$ which is the basis for $\mathbb{Q}(\omega)$.

## Q2

Define a substitution function $\sigma_\omega$
$$\sigma_\omega(a(x)) = a(\omega)$$
$\sigma_\omega$ is a homomorphism because
\begin{align*}
\sigma_\omega(a(x)b(x)) &= a(\omega)b(\omega) \\
    &= \sigma_\omega(a(x))\sigma_\omega(b(x))
\end{align*}
Which has a kernel of
\begin{align*}
\ker \sigma_\omega &= \{ a(x) : \sigma_\omega(a(x)) = a(\omega) = 0 \} \\
    &= J
\end{align*}
The kernel of any homomorphism is an ideal. In $F[x]$ every ideal is a principal ideal so $J = \langle p(x) \rangle$. So $p(x)$ is a polynomial of lowest degree among all nonzero polynomials in $J$. Hence it is irreducible.

When $n$ is prime, then
$$x^{n - 1} + x^{n - 2} + \cdots + x + 1$$
is irreducible. Therefore $p(x) = x^{n - 1} + \cdots + 1$ and $p(\omega) = 0$.
Since
$$\mathbb{Q}(\omega) \cong \mathbb{Q}[x] / \langle p(x) \rangle$$
Then $$[\mathbb{Q}(\omega):\mathbb{Q}] = \deg p(x) = n - 1$$

## Q3

$$p(\omega) = 0 \implies \omega^{n - 1} = -(\omega^{n - 2} + \cdots + \omega + 1)$$

## Q4

### n = 6

$$x^6 - 1 = (x^3 - 1)(x^3 + 1)$$

The roots are $1, s, s^2$ and $-1, -s, -s^2$ respectively where $s$ is the third root of unity.

But from above we know that $s^2 + s + 1 = 0 \implies s^2 = -(s + 1)$ and $s^2 \in \mathbb{Q}(s)$, so $\mathbb{Q}(\omega) = \mathbb{Q}(s)$ with basis $\{ 1, s \}$.

\begin{align*}
[\mathbb{Q}(\omega):\mathbb{Q}] &= [\mathbb{Q}(s): \mathbb{Q}] \\
    &= 2
\end{align*}

### n = 7

$n = 7$ is prime so $[\mathbb{Q}(\omega): \mathbb{Q}] = 6$.

### n = 8

\begin{align*}
x^8 - 1 &= (x^4 - 1)(x^4 + 1) \\
    &= (x^2 - 1)(x^2 + 1)(x^4 + 1)
\end{align*}

With roots $-1, 1$ and $i, -i$ for $(x^2 - 1)$ and $(x^2 + 1)$ respectively.

The 4th roots of $-1$ are $\pm \frac{1}{\sqrt{2}} \pm \frac{i}{\sqrt{2}}$.

$\mathbb{Q}(\omega) = \mathbb{Q}(\sqrt{2}, i)$ with a basis $\{ 1, \sqrt{2}, i, \sqrt{2}i \}$ and
$$[\mathbb{Q}(\omega):\mathbb{Q}] = [\mathbb{Q}(\sqrt{2}, i) : \mathbb{Q}] = 4$$

## Q5

$$\forall r \in \{ 1, 2, \dots, n - 1 \}, (\sqrt[n]{a} \omega^r)^n = 1$$

$$| \{ \sqrt[n]{a} \omega^r : r \in \{ 0, 1, \dots, n - 1 \} \} | = n$$

## Q6

The basis of $\mathbb{Q}(\omega, \sqrt[n]{a})$ is the set $\{ \omega^i (\sqrt[n]{a})^j \}$ where $i, j \in \{ 0, 1, \dots, n - 1 \}$, which contains the ideal for $\sigma(c) = x^n - 1$, which is $J = \{ \sqrt[n]{a}, \sqrt[n]{a} \omega, \dots, \sqrt[n]{a} \omega^{n - 1} \}$.

## Q7

The degree of $[\mathbb{Q}(\omega, \sqrt[3]{2}):\mathbb{Q}] = [\mathbb{Q}(\omega, \sqrt[3]{2}):\mathbb{Q}(\sqrt[3]{2})][\mathbb{Q}(\sqrt[3]{2}:\mathbb{Q}] = 2 \times 3 = 6$.

You can calculate $\cos (\pi / 3)$ and $\sin (\pi / 3)$ by splitting an equilateral triangle with unit sides in half. The sum of a triangle's angles will always be $\pi$, and so each corner of the equilateral triangle will be $(\pi / 3)$. Use pythagoreas theorem to calculate the midline as $o^2 = 1^2 - (\frac{1}{2})^2$.

Using wolfram alpha, we see that the cube roots of 1 are $1, -\frac{1}{2} + \frac{\sqrt{3}}{2} i, -\frac{1}{2} - \frac{\sqrt{3}}{2} i$.

$$\mathbb{Q}(\omega, \sqrt[3]{2}) = \mathbb{Q}(i\sqrt{3}, \sqrt[3]{2})$$

## Q8

Let $s$ be the nth root of $a$ in $K$, then it is the root of $x^n - a$. Then $\sqrt[n]{a}$ is also a root of this polynomial.

Fixing $\mathbb{Q}$, there is an isomorphism from $\mathbb{Q}(a) \rightarrow \mathbb{Q}(\sqrt[n]{a})$. Since $a(h(c)) = 0$, and the function is an isomorphism mapping one to one and onto, we can say that $h(x)$ permutes the roots $c$ of $x^n - a$. So we can see that $\mathbb{Q}(a) = \mathbb{Q}(\sqrt[n]{a})$, and that $K$ contains all roots of $x^n - a$.

